refined ret/malloc/alloca/store/load/bop/gep/cast/call.
git-svn-id: https://webdav.seas.upenn.edu/svn/sol/vol@3452 eef5ea85-cc2e-0410-bd84-0fae1f012da8

src/Transforms/promotable_props.v
@@ -82,8 +82,8 @@ Definition wf_alloca_GVs (maxb:Values.block) (pinfo:PhiInfo) TD Mem
   (gvsa:GenericValue) (als:list Values.block) : Prop :=
 (exists mb, gvsa = ($ (blk2GV TD mb) # (typ_pointer (PI_typ pinfo)) $) /\
    In mb als /\ maxb < mb) /\
-(forall gptr gvs1, 
-   mload TD Mem gptr (PI_typ pinfo) (PI_align pinfo) = Some gvs1 ->
+(forall gptr gvs1 ty al, 
+   mload TD Mem gptr ty al = Some gvs1 ->
    no_alias gvs1 gvsa) /\
 exists gv,
   mload TD Mem gvsa (PI_typ pinfo) (PI_align pinfo) = Some gv.
@@ -129,18 +129,23 @@ let '(Opsem.mkEC f b cs tmn lc als) := ec in
 else True)
 /\ wf_lc M lc.
 
+Definition wf_ECStack_head_in_tail (maxb:Values.block) (pinfo:PhiInfo) TD M 
+  (lc:DGVMap) (ec0:fdef * DGVMap) : Prop :=
+forall gvsa,
+  fst ec0 = PI_f pinfo ->
+  lookupAL _ (snd ec0) (PI_id pinfo) = Some gvsa ->
+  (exists mb, gvsa = ($ (blk2GV TD mb) # (typ_pointer (PI_typ pinfo)) $) /\ 
+    maxb < mb < Mem.nextblock M) /\
+  (forall id1 gvs1, 
+    lookupAL _ lc id1 = Some gvs1 -> 
+    no_alias gvs1 gvsa) /\
+  (forall gptr t al gvs1, 
+    mload TD M gptr t al = Some gvs1 -> 
+    no_alias gvs1 gvsa).
+
 Definition wf_ECStack_head_tail (maxb:Values.block) (pinfo:PhiInfo) TD M 
   (lc:DGVMap) (ecs':list (fdef * DGVMap)) : Prop :=
-  forall ec0 gvsa, 
-    In ec0 ecs' ->
-    fst ec0 = PI_f pinfo ->
-    lookupAL _ (snd ec0) (PI_id pinfo) = Some gvsa ->
-    (forall id1 gvs1, 
-      lookupAL _ lc id1 = Some gvs1 -> 
-      no_alias gvs1 gvsa) /\
-    (forall gptr gvs1, 
-      mload TD M gptr (PI_typ pinfo) (PI_align pinfo) = Some gvs1 -> 
-      no_alias gvs1 gvsa).
+  forall ec0, In ec0 ecs' -> wf_ECStack_head_in_tail maxb pinfo TD M lc ec0.
 
 Fixpoint wf_ECStack (maxb:Values.block) (pinfo:PhiInfo) TD M (ecs:Opsem.ECStack)
   : Prop :=
@@ -236,61 +241,128 @@ Proof.
         destruct Hin0 as [Hin0 | Hin0]; subst; try congruence; auto.
 Qed.
 
-Lemma free_preserves_mload_inv: forall TD Mem' gptr ty al gvsa Mem mptr0
-  (H1 : mload TD Mem' gptr ty al = ret gvsa)
-  (H2 : free TD Mem mptr0 = ret Mem'),
-  mload TD Mem gptr ty al = ret gvsa.
+Lemma preservation_helper1: forall los nts Ps S F l1 ps1 cs1' c0 tmn ifs
+  (HwfS : wf_system ifs S)
+  (HMinS : moduleInSystemB (module_intro los nts Ps) S = true)
+  (HFinPs : InProductsB (product_fdef F) Ps = true)
+  (HBinF : blockInFdefB (block_intro l1 ps1 (cs1' ++ [c0]) tmn) F = true),
+  ~ In (getCmdLoc c0) (getCmdsLocs cs1').
 Proof.
   intros.
-  apply mload_inv in H1.
-  destruct H1 as [b [ofs [m [mc [J1 [J2 J3]]]]]]; subst.
-  unfold mload. simpl. rewrite J2.
-  apply free_inv in H2.
-  destruct H2 as [blk' [ofs' [hi [lo [J4 [J5 [J6 J7]]]]]]].
-  admit. (* Mem Props *)
+  eapply wf_system__uniq_block with (f:=F) in HwfS; eauto.
+  simpl in HwfS.
+  apply NoDup_inv in HwfS.
+  destruct HwfS as [_ J].
+  apply NoDup_inv in J.
+  destruct J as [J _].
+  rewrite getCmdsLocs_app in J.
+  simpl in J.
+  apply NoDup_last_inv in J. auto.
 Qed.
 
-Lemma free_preserves_wf_ECStack_head_tail : forall maxb pinfo TD M M' lc mptr0
-  (Hfree: free TD M mptr0 = ret M') ECs 
-  (Hwf: wf_ECStack_head_tail maxb pinfo TD M lc ECs),
-  wf_ECStack_head_tail maxb pinfo TD M' lc ECs.
+Lemma preservation_helper2: forall los nts Ps S F l1 ps1 cs1' c0 tmn ifs c cs
+  (HwfS : wf_system ifs S)
+  (HMinS : moduleInSystemB (module_intro los nts Ps) S = true)
+  (HFinPs : InProductsB (product_fdef F) Ps = true)
+  (HBinF : blockInFdefB 
+            (block_intro l1 ps1 (cs1' ++ [c0] ++ [c] ++ cs) tmn) F = true),
+  NoDup (getCmdsLocs (cs1' ++ [c0] ++ [c] ++ cs)).
 Proof.
-  unfold wf_ECStack_head_tail.
   intros.
-  eapply Hwf in H1; eauto.
-  destruct H1 as [J1 J2].
+  eapply wf_system__uniq_block with (f:=F) in HwfS; eauto.
+  simpl in HwfS.
+  apply NoDup_inv in HwfS.
+  destruct HwfS as [_ J].
+  apply NoDup_inv in J.
+  destruct J as [J _]. auto.
+Qed.
+
+Definition inscope_of_pc f b cs tmn : option (list id) :=
+  match cs with
+  | nil => inscope_of_tmn f b tmn
+  | c::_ => inscope_of_cmd f b c
+  end.
+
+Lemma impure_cmd_non_updated_preserves_wf_EC : forall maxb pinfo TD M M' lc F B 
+  als tmn cs c0 l1 ps1 cs1' ifs S
+  (Heq: B = block_intro l1 ps1 (cs1' ++ c0 :: cs) tmn)
+  (HwfS: wf_system ifs S) los nts (Heq': TD = (los, nts)) Ps
+  (HMinS: moduleInSystemB (module_intro los nts Ps) S = true)
+  (HFinPs: InProductsB (product_fdef F) Ps = true)
+  (HBinF: blockInFdefB B F = true)
+  (Hid : getCmdID c0 = None)
+  (Hwfdefs: forall ids0,
+              F = (PI_f pinfo) ->
+              inscope_of_pc F B (c0::cs) tmn = Some ids0 ->
+              wf_defs maxb pinfo TD M lc ids0 als ->
+              wf_defs maxb pinfo TD M' lc ids0 als)
+  (Hwflc: wf_lc M lc -> wf_lc M' lc)
+  (HwfEC: wf_ExecutionContext maxb pinfo TD M 
+            {| Opsem.CurFunction := F;
+               Opsem.CurBB := B;
+               Opsem.CurCmds := c0 :: cs;
+               Opsem.Terminator := tmn;
+               Opsem.Locals := lc;
+               Opsem.Allocas := als |}),
+  wf_ExecutionContext maxb pinfo TD M'
+    {| Opsem.CurFunction := F;
+       Opsem.CurBB := B;
+       Opsem.CurCmds := cs;
+       Opsem.Terminator := tmn;
+       Opsem.Locals := lc;
+       Opsem.Allocas := als |}.
+Proof.
+  simpl. intros.
+  destruct HwfEC as [J1 J2].
   split; auto.
-    intros.
-    eapply free_preserves_mload_inv in H1; eauto.
+  destruct (fdef_dec (PI_f pinfo) F); subst; auto.
+  remember (inscope_of_cmd (PI_f pinfo) 
+    (block_intro l1 ps1 (cs1' ++ c0 :: cs) tmn) c0) as R1. 
+  assert (HeqR1':=HeqR1).
+  unfold inscope_of_cmd, inscope_of_id in HeqR1'.
+
+  destruct R1; try solve [inversion J1].
+  repeat (split; try solve [auto]).
+      destruct cs; simpl_env in *.
+      SSSSCase "cs = nil".
+        assert (~ In (getCmdLoc c0) (getCmdsLocs cs1')) 
+          as Hnotin.
+          eapply preservation_helper1; eauto.
+
+        apply inscope_of_cmd_tmn in HeqR1; auto.
+        destruct HeqR1 as [ids2 [J1' J2']].
+        rewrite <- J1'.
+        assert (In c0 (cs1' ++ [c0])) as HinCs.
+          apply in_or_app. right. simpl. auto.
+        assert (Hwfc := HBinF).
+        eapply wf_system__wf_cmd with (c:=c0) in Hwfc; 
+          eauto.
+        assert (HwfF:=HFinPs). eapply wf_system__wf_fdef in HwfF; eauto.
+        rewrite Hid in J2'. 
+        eapply wf_defs_eq; eauto.       
+
+      SSSSCase "cs <> nil".
+        assert (NoDup (getCmdsLocs (cs1' ++ [c0] ++ [c] ++ cs))) 
+          as Hnodup.
+          eapply preservation_helper2; eauto.
+
+        apply inscope_of_cmd_cmd in HeqR1; auto.
+        destruct HeqR1 as [ids2 [J1' J2']].        
+        rewrite <- J1'.
+        assert (In c0 (cs1' ++ [c0] ++ [c] ++ cs)) 
+          as HinCs.
+          apply in_or_app. right. simpl. auto.
+        assert (Hwfc := HBinF).
+        eapply wf_system__wf_cmd with (c:=c0) in Hwfc; 
+          eauto.
+        rewrite Hid in J2'. 
+        eapply wf_defs_eq; eauto.
 Qed.
 
-Lemma free_preserves_wf_lc: forall TD Mem' Mem mptr0 lc
-  (H2 : free TD Mem mptr0 = ret Mem')
-  (Hwf: wf_lc Mem lc),
-  wf_lc Mem' lc.
-Proof.
-  unfold wf_lc.
-  intros.
-  apply Hwf in H.
-  apply free_inv in H2.
-  destruct H2 as [blk' [ofs' [hi [lo [J4 [J5 [J6 J7]]]]]]].
-  admit. (* Mem Props *)
-Qed.
-(*
-Lemma free_allocas_preserves_mload: forall TD Mem als Mem' t al gv mb
-  (H0 : ~ In mb als)
-  (H1 : free_allocas TD Mem als = ret Mem')
-  (H2 : mload TD Mem ($ blk2GV TD mb # typ_pointer t $) t al = ret gv),
-  mload TD Mem' ($ blk2GV TD mb # typ_pointer t $) t al = ret gv.
+(* We need a generic proof for this one and the one for atom *)
+Lemma NoDup_disjoint : forall (l1 l2 : list Z) (i0 : Z),
+  NoDup (l1 ++ l2) -> In i0 l2 -> ~ In i0 l1.
 Admitted.
-*)
-
-Definition wf_use (pinfo:PhiInfo) (ids0:list id) (v:value) :=
-used_in_value (PI_id pinfo) v = false /\
-match v with
-| value_const _ => True
-| value_id vid => In vid ids0
-end.
 
 Lemma wf_globals_disjoint_with_runtime_alloca: forall maxb gl g td c0 mb t
   (Hwfg: wf_globals maxb gl)
@@ -299,236 +371,9 @@ Lemma wf_globals_disjoint_with_runtime_alloca: forall maxb gl g td c0 mb t
   no_alias g ($ blk2GV td mb # typ_pointer t $).
 Admitted.
 
-Lemma free_preserves_mload: forall TD Mem Mem' t al gv gptr gvsa
-  (H0 : no_alias gptr gvsa)
-  (H1 : free TD Mem gptr = ret Mem')
-  (H2 : mload TD Mem gvsa t al = ret gv),
-  mload TD Mem' gvsa t al = ret gv.
-Proof.
-  intros.
-  apply free_inv in H1.
-  destruct H1 as [blk [ofs [hi [lo [J4 [J5 [J6 J7]]]]]]].
-Admitted.
-
-Lemma free_preserves_wf_defs : forall maxb pinfo TD M  
-  M' lc1 mptr0 mptrs gl v als ids0 lc2
-  (Hwfu: wf_use pinfo ids0 v)
-  (Hgetop: Opsem.getOperandValue TD v lc1 gl = ret mptrs)
-  (Hin: mptr0 @ mptrs)
-  (Hwflc: wf_lc M lc1) (Hwfgl: wf_globals maxb gl)
-  (Hfree: free TD M mptr0 = ret M')
-  (Hwf: wf_defs maxb pinfo TD M lc2 ids0 als),
-  wf_defs maxb pinfo TD M' lc2 ids0 als.
-Proof.
-  intros. unfold wf_defs. 
-  intros gvsa Hpindom Hlkp.
-  assert (Hlkp':=Hlkp).
-  apply Hwf in Hlkp'; auto.
-  destruct Hlkp' as [J1 J2].
-  split; auto.
-    destruct J1 as [J1 [J4 [gv J3]]].
-    split; auto.
-      split.
-        intros. eapply free_preserves_mload_inv in H; eauto.
-        clear J4. inv Hin.
-        assert (no_alias mptr0 gvsa) as J.
-          destruct Hwfu as [G1 G2].
-          destruct v; simpl in Hgetop.
-(*
-          apply J2 in Hgetop; auto.
-          unfold wf_non_alloca_GVs in Hgetop.
-          simpl in G1. 
-          destruct (id_dec i0 (PI_id pinfo)); subst; tinv G1; auto.
-
-          destruct J1 as [mb [J11 [J12 J13]]]; subst.
-          eapply wf_globals_disjoint_with_runtime_alloca; eauto.
-        exists gv. eapply free_preserves_mload; eauto.
-*)
-Admitted.
-
-Lemma free_preserves_wf_EC_tail : forall maxb pinfo TD M  
-  M' mptr0 mptrs gl v EC (Hwfpi: WF_PhiInfo pinfo) lc
-  (Hgetop: Opsem.getOperandValue TD v lc gl = ret mptrs)
-  (Hin: mptr0 @ mptrs)
-  (Hwflc: wf_lc M lc) (Hwfgl: wf_globals maxb gl)
-  (Hfree: free TD M mptr0 = ret M')
-  (Hwf: wf_ExecutionContext maxb pinfo TD M EC),
-  wf_ExecutionContext maxb pinfo TD M' EC.
-Proof.
-  destruct EC. simpl. intros.
-  destruct Hwf as [J1 J2].
-  eapply free_preserves_wf_lc in J2; eauto.
-  split; auto.
-    destruct (fdef_dec (PI_f pinfo) CurFunction); subst; auto.
-    destruct CurCmds.    
-      remember (inscope_of_tmn (PI_f pinfo) CurBB Terminator) as R.
-      destruct R; auto.
-      eapply free_preserves_wf_defs in Hfree; eauto.   
-        admit. (* v >> current pc && Hwfpi *)
-
-      remember (inscope_of_cmd (PI_f pinfo) CurBB c) as R.
-      destruct R; auto.
-      eapply free_preserves_wf_defs in Hfree; eauto.   
-        admit. (* v >> current pc && Hwfpi *)
-Qed.
-
-Lemma free_preserves_wf_ECStack : forall maxb pinfo TD M  
-  M' mptr0 mptrs gl v (Hwfpi: WF_PhiInfo pinfo) lc
-  (Hgetop: Opsem.getOperandValue TD v lc gl = ret mptrs)
-  (Hin: mptr0 @ mptrs)
-  (Hwflc: wf_lc M lc) (Hwfgl: wf_globals maxb gl)
-  (Hfree: free TD M mptr0 = ret M') ECs
-  (Hwf: wf_ECStack maxb pinfo TD M ECs),
-  wf_ECStack maxb pinfo TD M' ECs.
-Proof.
-  induction ECs; simpl; intros; auto.
-    destruct Hwf as [J1 [J2 J3]].
-    split.
-      eapply free_preserves_wf_EC_tail; eauto.
-    split; eauto.
-      eapply free_preserves_wf_ECStack_head_tail; eauto.
-Qed.
-
-Lemma free_preserves_wf_EC : forall maxb pinfo TD M  
-  M' lc mptr0 mptrs gl v F B id0 t als tmn cs
-  (Hgetop: Opsem.getOperandValue TD v lc gl = ret mptrs)
-  (Hin: mptr0 @ mptrs)
-  (Hwflc: wf_lc M lc) (Hwfgl: wf_globals maxb gl)
-  (Hfree: free TD M mptr0 = ret M') 
-  (HwfEC: wf_ExecutionContext maxb pinfo TD M 
-            {| Opsem.CurFunction := F;
-               Opsem.CurBB := B;
-               Opsem.CurCmds := insn_free id0 t v :: cs;
-               Opsem.Terminator := tmn;
-               Opsem.Locals := lc;
-               Opsem.Allocas := als |}),
-  wf_ExecutionContext maxb pinfo TD M'
-   {| Opsem.CurFunction := F;
-      Opsem.CurBB := B;
-      Opsem.CurCmds := cs;
-      Opsem.Terminator := tmn;
-      Opsem.Locals := lc;
-      Opsem.Allocas := als |}.
-Admitted.
-
-Lemma free_preserves_wf_Mem : forall maxb TD M M' lc mptr0 mptrs gl v
-  (Hgetop: Opsem.getOperandValue TD v lc gl = ret mptrs)
-  (Hin: mptr0 @ mptrs)
-  (Hwflc: wf_lc M lc) (Hwfgl: wf_globals maxb gl)
-  (Hfree: free TD M mptr0 = ret M') 
-  (Hwf: wf_Mem maxb TD M),
-  wf_Mem maxb TD M'.
-Admitted.
-
-Lemma free_preserves_wf_als : forall maxb TD M M' mptr0 als
-  (Hfree: free TD M mptr0 = ret M') 
-  (Hwf: wf_als maxb M als),
-  wf_als maxb M' als.
-Admitted.
-
-Lemma free_allocas_preserves_mload_inv: forall TD Mem' gptr ty al gvsa Mem als
-  (H1 : mload TD Mem' gptr ty al = ret gvsa)
-  (H2 : free_allocas TD Mem als = ret Mem'),
-  mload TD Mem gptr ty al = ret gvsa.
-Proof.
-Admitted.
-
-Lemma free_allocas_preserves_mload: forall TD Mem als Mem' t al gv mb
-  (H0 : ~ In mb als)
-  (H1 : free_allocas TD Mem als = ret Mem')
-  (H2 : mload TD Mem ($ blk2GV TD mb # typ_pointer t $) t al = ret gv),
-  mload TD Mem' ($ blk2GV TD mb # typ_pointer t $) t al = ret gv.
-Admitted.
-
-(* We need a generic proof for this one and the one for atom *)
-Lemma NoDup_disjoint : forall (l1 l2 : list Z) (i0 : Z),
-  NoDup (l1 ++ l2) -> In i0 l2 -> ~ In i0 l1.
-Admitted.
-
-Lemma free_allocas_preserves_wf_alloca: forall maxb pinfo TD Mem gvsa als0 als Mem',
-  wf_alloca_GVs maxb pinfo TD Mem gvsa als0 ->
-  NoDup (als ++ als0) ->
-  free_allocas TD Mem als = ret Mem' ->
-  wf_alloca_GVs maxb pinfo TD Mem' gvsa als0.
-Proof.
-  intros.
-  unfold wf_alloca_GVs in *.
-  destruct H as [J1 [J2 J3]].
-  split; auto.
-  split.
-    intros gptr gvs1 J.  
-    eapply free_allocas_preserves_mload_inv in J; eauto.
-
-    destruct J3 as [gv J3].
-    exists gv.
-    destruct J1 as [mb [J11 [J12 J13]]]; subst.
-    eapply free_allocas_preserves_mload; eauto.
-    eapply NoDup_disjoint in H0; eauto.
-Qed.
-
-Lemma free_allocas_preserves_wf_defs: forall maxb pinfo TD Mem lc' l0 als0 als Mem',
-  wf_defs maxb pinfo TD Mem lc' l0 als0 ->
-  NoDup (als ++ als0) ->
-  free_allocas TD Mem als = ret Mem' ->
-  wf_defs maxb pinfo TD Mem' lc' l0 als0.
-  (* This is only true if als is always disjoint with pinfo.id *) 
-Proof.
-  intros. unfold wf_defs in *. intros.
-  apply H in Hlkp; auto. clear H.
-  destruct Hlkp as [J1 J2]. 
-  split; eauto using free_allocas_preserves_wf_alloca.
-Qed.
-
 Lemma undef_disjoint_with_runtime_alloca: forall g td mb t1 t2
   (Hc2g : ret g = gundef td t1),
   no_alias g ($ blk2GV td mb # typ_pointer t2 $).
-Admitted.
-
-Lemma free_allocas_preserves_wf_lc: forall td Mem als Mem' lc,
-  wf_lc Mem lc -> free_allocas td Mem als = ret Mem' -> wf_lc Mem' lc.
-Admitted.
-
-Lemma returnUpdateLocals__wf_lc: forall maxb td Result (lc:DGVMap) gl c' 
-  lc' Mem lc''
-  (H1 : Opsem.returnUpdateLocals td c' Result lc lc' gl = ret lc'')
-  (Hwflc1 : wf_lc Mem lc) (Hwflc2 : wf_lc Mem lc')
-  (Hwfg : wf_globals maxb gl) (Hgbound : maxb < Mem.nextblock Mem),
-  wf_lc Mem lc''.
-Admitted.
-
-Lemma free_allocas_preserves_wf_ECStack: forall maxb pinfo td Mem als Mem' ECs,
-  wf_ECStack maxb pinfo td Mem ECs ->
-  free_allocas td Mem als = ret Mem' ->
-  NoDup (als ++ (flat_map
-                  (fun ec : Opsem.ExecutionContext =>
-                   let '{| Opsem.Allocas := als |} := ec in als)
-                   ECs)) ->
-  wf_ECStack maxb pinfo td Mem' ECs.
-Admitted.
-
-Lemma wf_ECStack_head_tail__inv: forall maxb pinfo TD M lc ec1 ecs2,
-  wf_ECStack_head_tail maxb pinfo TD M lc (ec1::ecs2) ->
-  wf_ECStack_head_tail maxb pinfo TD M lc ecs2.
-Admitted.
-
-Lemma free_allocas_preserves_wf_ECStack_head_tail : forall maxb pinfo td M M' 
-  lc als lc' F' lc'' ECs gl Result c',
-  free_allocas td M als = ret M' ->
-  Opsem.returnUpdateLocals td c' Result lc lc' gl = ret lc'' ->
-  wf_ECStack_head_tail maxb pinfo td M lc ((F', lc')::ECs) ->
-  wf_ECStack_head_tail maxb pinfo td M lc' ECs ->
-  wf_ECStack_head_tail maxb pinfo td M' lc'' ECs.
-Admitted.
-
-Lemma free_allocas_preserves_wf_Mem: forall maxb td Mem als Mem',
-  wf_Mem maxb td Mem -> free_allocas td Mem als = ret Mem' -> 
-  wf_Mem maxb td Mem'.
-Admitted.
-
-Lemma free_allocas_preserves_wf_als : forall maxb TD M M' als als0
-  (Hfree: free_allocas TD M als0 = ret M') 
-  (Hwf: wf_als maxb M als),
-  wf_als maxb M' als.
 Admitted.
 
 Lemma preservation_return_helper: forall (g : GVsT DGVs) pinfo lc' Mem'
@@ -554,7 +399,7 @@ Proof.
   assert (Hlkp':=Hlkp).
   apply Hinscope2 in Hlkp'; auto.
   destruct Hlkp' as [[[mb [EQ [Hin Hbound]]] _] _]; subst.
-  edestruct Hfr1 as [G _]; simpl; eauto.
+  edestruct Hfr1 with (ec0:=(PI_f pinfo, lc')) as [_ [G _]]; simpl; eauto.
   clear Hfr1.
   simpl in G.
   Local Transparent lift_op1. simpl in HeqR2.
@@ -584,6 +429,96 @@ Qed.
 
 Ltac SSSSSCase name := Case_aux subsubsubsubsubcase name.
 Ltac SSSSSSCase name := Case_aux subsubsubsubsubsubcase name.
+
+Lemma free_allocas_preserves_mload_inv: forall TD Mem' gptr ty al gvsa Mem als
+  (H1 : mload TD Mem' gptr ty al = ret gvsa)
+  (H2 : free_allocas TD Mem als = ret Mem'),
+  mload TD Mem gptr ty al = ret gvsa.
+Proof.
+Admitted.
+
+Lemma free_allocas_preserves_mload: forall TD Mem als Mem' t al gv mb
+  (H0 : ~ In mb als)
+  (H1 : free_allocas TD Mem als = ret Mem')
+  (H2 : mload TD Mem ($ blk2GV TD mb # typ_pointer t $) t al = ret gv),
+  mload TD Mem' ($ blk2GV TD mb # typ_pointer t $) t al = ret gv.
+Admitted.
+
+Lemma free_allocas_preserves_wf_alloca: forall maxb pinfo TD Mem gvsa als0 als Mem',
+  wf_alloca_GVs maxb pinfo TD Mem gvsa als0 ->
+  NoDup (als ++ als0) ->
+  free_allocas TD Mem als = ret Mem' ->
+  wf_alloca_GVs maxb pinfo TD Mem' gvsa als0.
+Proof.
+  intros.
+  unfold wf_alloca_GVs in *.
+  destruct H as [J1 [J2 J3]].
+  split; auto.
+  split.
+    intros gptr gvs1 ty al J.  
+    eapply free_allocas_preserves_mload_inv in J; eauto.
+
+    destruct J3 as [gv J3].
+    exists gv.
+    destruct J1 as [mb [J11 [J12 J13]]]; subst.
+    eapply free_allocas_preserves_mload; eauto.
+    eapply NoDup_disjoint in H0; eauto.
+Qed.
+
+Lemma free_allocas_preserves_wf_defs: forall maxb pinfo TD Mem lc' l0 als0 als Mem',
+  wf_defs maxb pinfo TD Mem lc' l0 als0 ->
+  NoDup (als ++ als0) ->
+  free_allocas TD Mem als = ret Mem' ->
+  wf_defs maxb pinfo TD Mem' lc' l0 als0.
+  (* This is only true if als is always disjoint with pinfo.id *) 
+Proof.
+  intros. unfold wf_defs in *. intros.
+  apply H in Hlkp; auto. clear H.
+  destruct Hlkp as [J1 J2]. 
+  split; eauto using free_allocas_preserves_wf_alloca.
+Qed.
+
+Lemma free_allocas_preserves_wf_lc: forall td Mem als Mem' lc,
+  wf_lc Mem lc -> free_allocas td Mem als = ret Mem' -> wf_lc Mem' lc.
+Admitted.
+
+Lemma returnUpdateLocals__wf_lc: forall maxb td Result (lc:DGVMap) gl c' 
+  lc' Mem lc''
+  (H1 : Opsem.returnUpdateLocals td c' Result lc lc' gl = ret lc'')
+  (Hwflc1 : wf_lc Mem lc) (Hwflc2 : wf_lc Mem lc')
+  (Hwfg : wf_globals maxb gl) (Hgbound : maxb < Mem.nextblock Mem),
+  wf_lc Mem lc''.
+Admitted.
+
+Lemma free_allocas_preserves_wf_ECStack: forall maxb pinfo td Mem als Mem' ECs,
+  wf_ECStack maxb pinfo td Mem ECs ->
+  free_allocas td Mem als = ret Mem' ->
+  NoDup (als ++ (flat_map
+                  (fun ec : Opsem.ExecutionContext =>
+                   let '{| Opsem.Allocas := als |} := ec in als)
+                   ECs)) ->
+  wf_ECStack maxb pinfo td Mem' ECs.
+Admitted.
+
+Lemma free_allocas_preserves_wf_ECStack_head_tail : forall maxb pinfo td M M' 
+  lc als lc' F' lc'' ECs gl Result c',
+  free_allocas td M als = ret M' ->
+  Opsem.returnUpdateLocals td c' Result lc lc' gl = ret lc'' ->
+  wf_ECStack_head_tail maxb pinfo td M lc ((F', lc')::ECs) ->
+  wf_ECStack_head_tail maxb pinfo td M lc' ECs ->
+  wf_ECStack_head_tail maxb pinfo td M' lc'' ECs.
+Admitted.
+
+Lemma free_allocas_preserves_wf_Mem: forall maxb td Mem als Mem',
+  wf_Mem maxb td Mem -> free_allocas td Mem als = ret Mem' -> 
+  wf_Mem maxb td Mem'.
+Admitted.
+
+Lemma free_allocas_preserves_wf_als : forall maxb TD M M' als als0
+  (Hfree: free_allocas TD M als0 = ret M') 
+  (Hwf: wf_als maxb M als),
+  wf_als maxb M' als.
+Admitted.
 
 Lemma preservation_return : forall maxb pinfo (HwfPI : WF_PhiInfo pinfo)  
   F B rid RetTy Result lc F' B' c' cs' tmn' lc' EC Mem als als' cfg
@@ -655,12 +590,7 @@ Local Opaque inscope_of_tmn inscope_of_cmd.
     remember (inscope_of_cmd 
       (PI_f pinfo) (block_intro l2 ps2 (cs2' ++ c' :: cs') tmn') c') as R2.
     destruct R2; try solve [inversion Hinscope2].
-(*
-    remember (inscope_of_tmn F
-               (block_intro l1 ps1 (cs1' ++ nil)(insn_return rid RetTy Result))
-               (insn_return rid RetTy Result)) as R1. 
-    destruct R1; try solve [inversion Hinscope1].
-*)
+
     remember (getCmdID c') as R.
     destruct c'; try solve [inversion H].
     assert (In (insn_call i0 n c t v p) 
@@ -686,15 +616,8 @@ Local Opaque inscope_of_tmn inscope_of_cmd.
     SSSSCase "cs' = nil".
       assert (~ In (getCmdLoc (insn_call i0 n c t v p)) (getCmdsLocs cs2')) 
         as Hnotin.
-        eapply wf_system__uniq_block with (f:=(PI_f pinfo)) in HwfSystem; eauto.        
-        simpl in HwfSystem.
-        apply NoDup_inv in HwfSystem.
-        destruct HwfSystem as [_ J].
-        apply NoDup_inv in J.
-        destruct J as [J _].
-        rewrite getCmdsLocs_app in J.
-        simpl in J.
-        apply NoDup_last_inv in J. auto.
+        eapply preservation_helper1; eauto.
+
       assert (HeqR2':=HeqR2).
       apply inscope_of_cmd_tmn in HeqR2; auto.
       destruct HeqR2 as [ids2 [J1 J2]].
@@ -725,12 +648,8 @@ Local Opaque inscope_of_tmn inscope_of_cmd.
     SSSSCase "cs' <> nil".
       assert (NoDup (getCmdsLocs (cs2' ++ [insn_call i0 n c t v p] ++ [c0] ++ 
         cs'))) as Hnodup.
-        eapply wf_system__uniq_block with (f:=PI_f pinfo) in HwfSystem; eauto.
-        simpl in HwfSystem.
-        apply NoDup_inv in HwfSystem.
-        destruct HwfSystem as [_ J].
-        apply NoDup_inv in J.
-        destruct J as [J _]. auto.
+        eapply preservation_helper2; eauto.
+
       assert (HeqR2':=HeqR2). simpl_env in HeqR2.
       apply inscope_of_cmd_cmd in HeqR2; auto.
       destruct HeqR2 as [ids2 [J1 J2]].        
@@ -825,18 +744,10 @@ Definition wf_GVs_in_EC (maxb:Values.block) (pinfo:PhiInfo) TD M
   (ec:Opsem.ExecutionContext)(id1:id)(gv1:GVsT DGVs) : Prop :=
 let '(Opsem.mkEC f b cs tmn lc als) := ec in
 (if (fdef_dec (PI_f pinfo) f) then 
-  match cs with
-  | nil => 
-    match inscope_of_tmn f b tmn with
-    | Some ids => wf_GVs maxb pinfo TD M lc ids als id1 gv1
-    | None => False
-    end
-  | c::_ =>
-    match inscope_of_cmd f b c with
-    | Some ids => wf_GVs maxb pinfo TD M lc ids als id1 gv1
-    | None => False
-    end
-  end 
+  forall ids0, 
+    inscope_of_pc f b cs tmn = Some ids0 ->
+    wf_defs maxb pinfo TD M lc ids0 als ->
+    wf_GVs maxb pinfo TD M lc ids0 als id1 gv1
 else True) /\
 (forall blk ofs, gv1 = mk_gptr blk ofs -> blk < Mem.nextblock M).
 
@@ -899,30 +810,17 @@ Local Opaque inscope_of_cmd inscope_of_tmn.
 Transparent inscope_of_cmd.
 
   unfold inscope_of_cmd, inscope_of_id in HeqR1'.
-  assert (uniqFdef (PI_f pinfo)) as HuniqF.
-    eapply wf_system__uniqFdef; eauto.
   destruct R1; try solve [inversion Hinscope1].
   repeat (split; try solve [auto]).
       assert (Hid':=Hid).
       symmetry in Hid.
       apply getCmdLoc_getCmdID in Hid.
       subst.
-      assert (cmdInBlockB c0 (block_intro l1 ps1 (cs1' ++ c0 :: cs) tmn) = true) 
-        as Hin.
-        simpl. apply In_InCmdsB. apply in_middle.
       destruct cs; simpl_env in *.
       SSSSCase "cs = nil".
         assert (~ In (getCmdLoc c0) (getCmdsLocs cs1')) as Hnotin.
           (* this lemma should be lifted to the top *)
-          eapply wf_system__uniq_block with (f:=PI_f pinfo) in HwfSystem; eauto.
-          simpl in HwfSystem.
-          apply NoDup_inv in HwfSystem.
-          destruct HwfSystem as [_ J].
-          apply NoDup_inv in J.
-          destruct J as [J _].
-          rewrite getCmdsLocs_app in J.
-          simpl in J.
-          apply NoDup_last_inv in J. auto.
+          eapply preservation_helper1; eauto.
 
         apply inscope_of_cmd_tmn in HeqR1; auto.
         destruct HeqR1 as [ids2 [J1 J2]].        
@@ -939,12 +837,8 @@ Transparent inscope_of_cmd.
       SSSSCase "cs <> nil".
         assert (NoDup (getCmdsLocs (cs1' ++ [c0] ++ [c] ++ cs))) as Hnodup.
           (* this lemma should be lifted to the top *)
-          eapply wf_system__uniq_block with (f:=PI_f pinfo) in HwfSystem; eauto.
-          simpl in HwfSystem.
-          apply NoDup_inv in HwfSystem.
-          destruct HwfSystem as [_ J].
-          apply NoDup_inv in J.
-          destruct J as [J _]. auto.
+          eapply preservation_helper2; eauto.
+
         apply inscope_of_cmd_cmd in HeqR1; auto.
         destruct HeqR1 as [ids2 [J1 J2]].        
         rewrite <- J1.
@@ -970,169 +864,167 @@ Transparent inscope_of_cmd inscope_of_tmn.
 Qed.
 
 Lemma BOP__wf_GVs_in_EC : forall (v : value) (v0 : value) (id1 : id) (bop0 : bop)
-  gvs3 TD bop0 sz0 lc gl EC Mem0 td pinfo maxb
+  gvs3 TD bop0 sz0 lc gl EC Mem0 td pinfo maxb (Hneq: id1 <> PI_id pinfo)
   (H11 : BOP TD lc gl bop0 sz0 v v0 = ret gvs3),
   wf_GVs_in_EC maxb pinfo td Mem0 EC id1 gvs3.
 Proof.
   intros. 
+  unfold wf_GVs_in_EC. destruct EC.
+  split.
+    destruct (fdef_dec (PI_f pinfo) CurFunction); subst; auto.
+    intros.
+    split; intros; subst; try congruence.
+      admit. (* BOP isnt ptr *)
+
+    intros. subst.
+    admit. (* BOP isnt ptr *)
+Qed.
+
+Definition wf_use_at_head (pinfo:PhiInfo) (ids0:list id) (v:value) :=
+used_in_value (PI_id pinfo) v = false /\
+match v with
+| value_const _ => True
+| value_id vid => In vid ids0
+end.
+
+Lemma operand__no_alias_with__head: forall maxb pinfo TD lc mptr0 mptrs gl v als
+  (Hgetop : Opsem.getOperandValue TD v lc gl = ret mptrs)
+  (Hin : mptr0 @ mptrs) (Hwfgl : wf_globals maxb gl) ids0 M
+  (Hwfu: wf_use_at_head pinfo ids0 v) (Hwf: wf_defs maxb pinfo TD M lc ids0 als)
+  (gvsa : GVsT DGVs) (Hpindom : In (PI_id pinfo) ids0)
+  (Hlkp : lookupAL (GVsT DGVs) lc (PI_id pinfo) = ret gvsa),
+  no_alias mptr0 gvsa.
+Proof.
+  intros.
+  apply Hwf in Hlkp; auto.
+  destruct Hlkp as [[J1 [J4 [gv J3]]] J2].
+  inv Hin.
+  destruct v; simpl in Hgetop.
+    destruct Hwfu as [Hwfu1 Hwfu2].        
+    apply J2 in Hgetop; auto.
+    unfold wf_non_alloca_GVs in Hgetop.
+    destruct (id_dec i0 (PI_id pinfo)); subst; auto.
+      inv Hwfu1. 
+      destruct (id_dec (PI_id pinfo) (PI_id pinfo)); try congruence.
+        inv H0.
+  
+    destruct J1 as [mb [J11 [J12 J13]]]; subst.
+    eapply wf_globals_disjoint_with_runtime_alloca; eauto.
+Qed.
+
+Lemma wf_globals__le_maxb: forall maxb gl td c0 
+  (Hwfg: wf_globals maxb gl) blk ofs
+  (Hc2g : ret mk_gptr blk ofs = @Opsem.const2GV DGVs td gl c0),
+  blk <= maxb.
 Admitted.
 
-Lemma CAST__wf_GVs_in_EC : forall (v : value) (v0 : value) (id1 : id)
-  gvs2 TD lc gl EC Mem0 td pinfo maxb castop0 t1 v1 t2
-  (H11 : Opsem.CAST TD lc gl castop0 t1 v1 t2 = ret gvs2),
-  wf_GVs_in_EC maxb pinfo td Mem0 EC id1 gvs2.
+Lemma operand__lt_nextblock: forall maxb TD M (lc:DGVMap) blk ofs gl
+  (Hwfgl : wf_globals maxb gl) v mptrs (Hlt: maxb < Mem.nextblock M)
+  (Hwflc: wf_lc M lc) 
+  (Hin: mk_gptr blk ofs @ mptrs) 
+  (Hgetop : Opsem.getOperandValue TD v lc gl = ret mptrs),
+  blk < Mem.nextblock M.
+Proof.
+  intros.
+  inv Hin.
+  destruct v; simpl in Hgetop.
+    apply Hwflc in Hgetop; auto.
+
+    eapply wf_globals__le_maxb in Hwfgl; eauto.
+    omega.
+Qed.     
+
+Lemma CAST__wf_GVs_in_EC : forall (v : value) (id1 : id)
+  gvs2 TD gl EC Mem pinfo maxb castop0 t1 t2 
+  (Hwflc: wf_lc Mem (@Opsem.Locals DGVs EC)) 
+  (Hwfgl: wf_globals maxb gl) (HwfM: maxb < Mem.nextblock Mem)
+  (Hwfv: forall ids0,
+         let '(Opsem.mkEC F B cs tmn _ _) := EC in
+         F = (PI_f pinfo) ->
+         inscope_of_pc F B cs tmn = Some ids0 ->
+         wf_use_at_head pinfo ids0 v)
+  (Hneq: id1 <> PI_id pinfo)
+  (H11 : Opsem.CAST TD (@Opsem.Locals DGVs EC) gl castop0 t1 v t2 
+           = ret gvs2),
+  wf_GVs_in_EC maxb pinfo TD Mem EC id1 gvs2.
 Proof.
   intros. 
-Admitted.
+  unfold wf_GVs_in_EC. destruct EC.
+  apply OpsemProps.CAST_inversion in H11.
+  destruct H11 as [gv1 [J1 J2]].
+  split.
+    destruct (fdef_dec (PI_f pinfo) CurFunction); subst; auto.
+    intros.
+    split; intros; subst; try congruence.
+      assert (H2':=H2).
+      apply H0 in H2; auto.
+      destruct H2 as [[J5 [J6 J3]] J4]; eauto.
+      eapply operand__no_alias_with__head with (als:=Allocas) (mptr0:=gv1)
+        (M:=Mem) in J1; eauto.
+        clear - J1 J2. admit. (* CAST is aliasing *)
 
-Lemma malloc_preserves_wf_ECStack_head_tail : forall maxb pinfo ECs TD M tsz gn 
-  align0 M' lc mb t id0,
-  malloc TD M tsz gn align0 = ret (M', mb) ->
-  wf_ECStack_head_tail maxb pinfo TD M lc ECs ->
-  wf_ECStack_head_tail maxb pinfo TD M' 
-    (updateAddAL (GVsT DGVs) lc id0
-        ($ blk2GV TD mb # typ_pointer t $)) ECs.
-Admitted.
-
-Lemma malloc_preserves_wf_ECStack : forall maxb pinfo ECs TD M tsz gn align0 M' 
-  mb,
-  malloc TD M tsz gn align0 = ret (M', mb) ->
-  wf_ECStack maxb pinfo TD M ECs ->
-  wf_ECStack maxb pinfo TD M' ECs.
-Admitted.
-
-Lemma malloc_preserves_wf_EC : forall maxb pinfo TD M tsz gn align0 M' mb 
-  als t id0 F B cs tmn lc v gns gl
-  (H : getTypeAllocSize TD t = ret tsz)
-  (H0 : Opsem.getOperandValue TD v lc gl = ret gns)
-  (H1 : gn @ gns)
-  (H2 : malloc TD M tsz gn align0 = ret (M', mb))
-  (HwfEC: wf_ExecutionContext maxb pinfo TD M 
-            {| Opsem.CurFunction := F;
-               Opsem.CurBB := B;
-               Opsem.CurCmds := insn_malloc id0 t v align0 :: cs;
-               Opsem.Terminator := tmn;
-               Opsem.Locals := lc;
-               Opsem.Allocas := als |}),
-  wf_ExecutionContext maxb pinfo TD M'
-   {| Opsem.CurFunction := F;
-      Opsem.CurBB := B;
-      Opsem.CurCmds := cs;
-      Opsem.Terminator := tmn;
-      Opsem.Locals := updateAddAL (GVsT DGVs) lc id0
-                        ($ blk2GV TD mb # typ_pointer t $);
-      Opsem.Allocas := als |}.
-Admitted.
-
-Lemma malloc_preserves_wf_Mem : forall maxb TD M tsz gn align0 M' mb,
-  malloc TD M tsz gn align0 = ret (M', mb) ->
-  wf_Mem maxb TD M ->
-  wf_Mem maxb TD M'.
-Admitted.
+    intros. subst.
+    assert (exists ofs', gv1 = mk_gptr blk ofs') as EQ. admit. (* CAST inv *)
+    destruct EQ as [ofs' EQ]; subst.
+    eapply operand__lt_nextblock in J1; eauto.
+Qed.
 
 Lemma wf_EC__wf_lc : forall maxb pinfo TD M EC,
   wf_ExecutionContext maxb pinfo TD M EC ->
   wf_lc M (Opsem.Locals EC).
 Admitted.
 
-Lemma alloca_preserves_wf_EC : forall maxb pinfo TD M tsz gn align0 M' mb 
-  als t id0 F B cs tmn lc v gns gl
-  (H : getTypeAllocSize TD t = ret tsz)
-  (H0 : Opsem.getOperandValue TD v lc gl = ret gns)
-  (H1 : gn @ gns)
-  (H2 : malloc TD M tsz gn align0 = ret (M', mb))
-  (HwfEC: wf_ExecutionContext maxb pinfo TD M 
-            {| Opsem.CurFunction := F;
-               Opsem.CurBB := B;
-               Opsem.CurCmds := insn_malloc id0 t v align0 :: cs;
-               Opsem.Terminator := tmn;
-               Opsem.Locals := lc;
-               Opsem.Allocas := als |}),
-  wf_ExecutionContext maxb pinfo TD M'
-   {| Opsem.CurFunction := F;
-      Opsem.CurBB := B;
-      Opsem.CurCmds := cs;
-      Opsem.Terminator := tmn;
-      Opsem.Locals := updateAddAL (GVsT DGVs) lc id0
-                        ($ blk2GV TD mb # typ_pointer t $);
-      Opsem.Allocas := mb :: als |}.
-Admitted.
-
-Lemma malloc_preserves_wf_als : forall maxb TD M M' tsz gn align0 mb als
-  (Hmalloc: malloc TD M tsz gn align0 = ret (M', mb)) 
-  (Hwf: wf_als maxb M als),
-  wf_als maxb M' (mb::als).
-Admitted.
-
 Lemma mload__wf_GVs_in_EC : forall (v : value) (v0 : value) (id1 : id) 
-  gvs3 TD t align0 (lc:DGVMap) gl EC Mem td pinfo maxb mp mps
-  (Hwflc: wf_lc Mem lc) (Hwfgl: wf_globals maxb gl)
-  (H : Opsem.getOperandValue td v lc gl = ret mps)
-  (H0 : mp @ mps)
-  (H1 : mload TD Mem mp t align0 = ret gvs3),
+  gvs3 t align0 EC Mem td pinfo maxb mp
+  (Hneq: id1 <> PI_id pinfo) (HwfM: wf_Mem maxb td Mem)
+  (H1 : mload td Mem mp t align0 = ret gvs3),
   wf_GVs_in_EC maxb pinfo td Mem EC id1 gvs3.
 Proof.
   intros. 
-Admitted.
+  unfold wf_GVs_in_EC. destruct EC.
+  split.
+    destruct (fdef_dec (PI_f pinfo) CurFunction); subst; auto.
+    intros.
+    split; intros; subst; try congruence.
+      apply H0 in H3; auto.
+      destruct H3 as [[J1 [J2 J3]] _]; eauto.
 
-Lemma mstore_preserves_wf_ECStack_head_tail : forall maxb pinfo ECs TD M 
-  gv1 align M' lc mp2 t,
-  mstore TD M mp2 t gv1 align = Some M' ->
-  wf_ECStack_head_tail maxb pinfo TD M lc ECs ->
-  wf_ECStack_head_tail maxb pinfo TD M' lc ECs.
-Admitted.
-
-Lemma mstore_preserves_wf_ECStack : forall maxb pinfo ECs TD M mp2 t gv1 align 
-  M', 
-  mstore TD M mp2 t gv1 align = Some M' ->
-  wf_ECStack maxb pinfo TD M ECs ->
-  wf_ECStack maxb pinfo TD M' ECs.
-Admitted.
-
-Lemma mstore_preserves_wf_EC : forall maxb pinfo TD M v1 gvs1 gv1 M'
-  als t id0 F B cs tmn (lc:DGVMap) gl align0 v2 mp2
-  (Hwflc: wf_lc M lc) (Hwfgl: wf_globals maxb gl)
-  (H0 : Opsem.getOperandValue TD v1 lc gl = Some gvs1)
-  (H1 : gv1 @ gvs1)
-  (H2 : mstore TD M mp2 t gv1 align0 = Some M')
-  (HwfEC: wf_ExecutionContext maxb pinfo TD M 
-            {| Opsem.CurFunction := F;
-               Opsem.CurBB := B;
-               Opsem.CurCmds := insn_store id0 t v1 v2 align0 :: cs;
-               Opsem.Terminator := tmn;
-               Opsem.Locals := lc;
-               Opsem.Allocas := als |}),
-  wf_ExecutionContext maxb pinfo TD M'
-   {| Opsem.CurFunction := F;
-      Opsem.CurBB := B;
-      Opsem.CurCmds := cs;
-      Opsem.Terminator := tmn;
-      Opsem.Locals := lc;
-      Opsem.Allocas := als |}.
-Admitted.
-
-Lemma mstore_preserves_wf_Mem : forall maxb TD M mp2 t gv1 align M',
-  mstore TD M mp2 t gv1 align = Some M' ->
-  wf_Mem maxb TD M ->
-  wf_Mem maxb TD M'.
-Admitted.
-
-Lemma mstore_preserves_wf_als : forall TD M mp2 t gv1 align M' maxb als
-  (Hst: mstore TD M mp2 t gv1 align = Some M') 
-  (Hwf: wf_als maxb M als),
-  wf_als maxb M' als.
-Admitted.
+    intros. subst.
+    destruct HwfM as [J1 J2]; eauto.
+Qed.
 
 Lemma GEP__wf_GVs_in_EC : forall (v : value) (v0 : value) (id1 : id) 
-  mp' TD t (lc:DGVMap) gl EC Mem td pinfo maxb (mp:GVsT DGVs) mps 
-  inbounds0 vidxs (Hwflc: wf_lc Mem lc) (Hwfgl: wf_globals maxb gl)
-  (H : Opsem.getOperandValue td v lc gl = ret mps)
-  (H0 : mp @ mps)
+  mp' TD t gl EC Mem td pinfo maxb (mp:GVsT DGVs) mps 
+  inbounds0 vidxs (Hwflc: wf_lc Mem (@Opsem.Locals DGVs EC)) 
+  (Hwfgl: wf_globals maxb gl) (HwfM: maxb < Mem.nextblock Mem)
+  (Hwfv: forall ids0,
+         let '(Opsem.mkEC F B cs tmn _ _) := EC in
+         F = (PI_f pinfo) ->
+         inscope_of_pc F B cs tmn = Some ids0 ->
+         wf_use_at_head pinfo ids0 v)
+  (H : Opsem.getOperandValue td v (Opsem.Locals EC) gl = ret mps)
+  (H0 : mp @ mps) (Hneq: id1 <> PI_id pinfo)
   (H1 : Opsem.GEP TD t mp vidxs inbounds0 = ret mp'),
   wf_GVs_in_EC maxb pinfo td Mem EC id1 mp'.
 Proof.
   intros. 
-Admitted.
+  unfold wf_GVs_in_EC. destruct EC.
+  split.
+    destruct (fdef_dec (PI_f pinfo) CurFunction); subst; auto.
+    intros.
+    split; intros; subst; try congruence.
+      assert (H5':=H5).
+      apply H3 in H5; auto.
+      destruct H5 as [[J1 [J2 J3]] J4]; eauto.
+      eapply operand__no_alias_with__head with (als:=Allocas) (mptr0:=mp)
+        (M:=Mem) in H; eauto.
+        clear - H1 H. admit. (* GEP is aliasing *)
+
+    intros. subst.
+    assert (exists ofs', mp = mk_gptr blk ofs') as EQ. admit. (* GEP inv *)
+    destruct EQ as [ofs' EQ]; subst.
+    eapply operand__lt_nextblock in H; eauto.
+Qed.
 
 Lemma initLocals_preserves_wf_ECStack_head_tail: forall Mem (lc:DGVMap) maxb TD 
   F ECs lc' gl (Hwflc1 : wf_lc Mem lc) pinfo gvs la lp
@@ -1256,6 +1148,832 @@ Lemma callExternalFun_preserves_wf_EC : forall maxb pinfo TD M M' rid
       Opsem.Allocas := als |}.
 Admitted.
 
+Lemma free_preserves_mload_inv: forall TD Mem' gptr ty al gvsa Mem mptr0
+  (H1 : mload TD Mem' gptr ty al = ret gvsa)
+  (H2 : free TD Mem mptr0 = ret Mem'),
+  mload TD Mem gptr ty al = ret gvsa.
+Proof.
+  intros.
+  apply mload_inv in H1.
+  destruct H1 as [b [ofs [m [mc [J1 [J2 J3]]]]]]; subst.
+  unfold mload. simpl. rewrite J2.
+  apply free_inv in H2.
+  destruct H2 as [blk' [ofs' [hi [lo [J4 [J5 [J6 J7]]]]]]].
+  admit. (* Mem Props *)
+Qed.
+
+Lemma free_preserves_wf_ECStack_head_tail : forall maxb pinfo TD M M' lc mptr0
+  (Hfree: free TD M mptr0 = ret M') ECs 
+  (Hwf: wf_ECStack_head_tail maxb pinfo TD M lc ECs),
+  wf_ECStack_head_tail maxb pinfo TD M' lc ECs.
+Proof.
+  unfold wf_ECStack_head_tail, wf_ECStack_head_in_tail.
+  intros.
+  eapply Hwf in H0; eauto.
+  destruct H0 as [[mb [J11 J12]] [J2 J3]]; subst.
+  split.
+    exists mb. split; auto. admit. (* Mem Prop *)
+  split; auto.
+    intros.
+    eapply free_preserves_mload_inv in H0; eauto.
+Qed.
+
+Lemma free_preserves_wf_lc: forall TD Mem' Mem mptr0
+  (H2 : free TD Mem mptr0 = ret Mem') lc
+  (Hwf: wf_lc Mem lc),
+  wf_lc Mem' lc.
+Proof.
+  unfold wf_lc.
+  intros.
+  apply Hwf in H.
+  apply free_inv in H2.
+  destruct H2 as [blk' [ofs' [hi [lo [J4 [J5 [J6 J7]]]]]]].
+  admit. (* Mem Props *)
+Qed.
+
+Definition wf_use_in_tail (pinfo:PhiInfo) (v:value) :=
+used_in_value (PI_id pinfo) v = false.
+
+Lemma free_preserves_mload: forall TD Mem Mem' t al gv gptr gvsa
+  (H0 : no_alias gptr gvsa)
+  (H1 : free TD Mem gptr = ret Mem')
+  (H2 : mload TD Mem gvsa t al = ret gv),
+  mload TD Mem' gvsa t al = ret gv.
+Proof.
+  intros.
+  apply free_inv in H1.
+  destruct H1 as [blk [ofs [hi [lo [J4 [J5 [J6 J7]]]]]]].
+  admit. (* Mem Props *)
+Admitted.
+
+Lemma operand__no_alias_with__tail: forall maxb pinfo TD M lc1 lc2 mptr0 gl
+  (Hwfgl : wf_globals maxb gl) v mptrs
+  (Hht : wf_ECStack_head_in_tail maxb pinfo TD M lc1 (PI_f pinfo, lc2))
+  (gvsa : GVsT DGVs) (Hin: mptr0 @ mptrs) 
+  (Hlkp : lookupAL (GVsT DGVs) lc2 (PI_id pinfo) = ret gvsa)
+  (Hgetop : Opsem.getOperandValue TD v lc1 gl = ret mptrs),
+  no_alias mptr0 gvsa.
+Proof.
+  intros.
+  inv Hin.
+  apply Hht in Hlkp; auto.
+  destruct Hlkp as [[mb [J11 J12]] [Hlkp _]]; subst.
+  destruct v; simpl in Hgetop.
+    apply Hlkp in Hgetop; auto.
+    eapply wf_globals_disjoint_with_runtime_alloca; eauto.
+      omega.
+Qed.
+
+Lemma free_preserves_wf_defs_in_tail : forall maxb pinfo TD M  
+  M' lc1 mptr0 mptrs gl v als lc2 
+  (Hgetop: Opsem.getOperandValue TD v lc1 gl = ret mptrs)
+  (Hin: mptr0 @ mptrs) (Hwfgl: wf_globals maxb gl)
+  (Hfree: free TD M mptr0 = ret M')
+  (Hht: wf_ECStack_head_in_tail maxb pinfo TD M lc1 (PI_f pinfo, lc2))
+  ids0 (Hwf: wf_defs maxb pinfo TD M lc2 ids0 als),
+  wf_defs maxb pinfo TD M' lc2 ids0 als.
+Proof.
+  intros. unfold wf_defs. 
+  intros gvsa Hpindom Hlkp.
+  assert (Hlkp':=Hlkp).
+  apply Hwf in Hlkp'; auto.
+  destruct Hlkp' as [J1 J2].
+  split; auto.
+    clear J2.
+    destruct J1 as [J1 [J4 [gv J3]]].
+    split; auto.
+      split.
+        intros. eapply free_preserves_mload_inv in H; eauto.
+        clear J4. 
+        assert (no_alias mptr0 gvsa) as J.
+          eapply operand__no_alias_with__tail; eauto.
+        exists gv. eapply free_preserves_mload; eauto.
+Qed.
+
+Lemma free_preserves_wf_defs_at_head : forall maxb pinfo TD M  
+  M' lc mptr0 mptrs gl v als
+  (Hgetop: Opsem.getOperandValue TD v lc gl = ret mptrs)
+  (Hin: mptr0 @ mptrs) (Hwfgl: wf_globals maxb gl)
+  (Hfree: free TD M mptr0 = ret M')
+  ids0 (Hwfu: wf_use_at_head pinfo ids0 v) 
+  (Hwf: wf_defs maxb pinfo TD M lc ids0 als),
+  wf_defs maxb pinfo TD M' lc ids0 als.
+Proof.
+  intros. unfold wf_defs. 
+  intros gvsa Hpindom Hlkp.
+  assert (no_alias mptr0 gvsa) as J.
+    eapply operand__no_alias_with__head; eauto.
+  assert (Hlkp':=Hlkp).
+  apply Hwf in Hlkp'; auto.
+  destruct Hlkp' as [J1 J2].
+  split; auto.
+    destruct J1 as [J1 [J4 [gv J3]]].
+    split; auto.
+      split.
+        intros. eapply free_preserves_mload_inv in H; eauto.
+        exists gv. eapply free_preserves_mload; eauto.
+Qed.
+
+Lemma impure_cmd_preserves_wf_EC_tail : forall maxb pinfo TD M  
+  M' EC (Hwfpi: WF_PhiInfo pinfo) 
+  (Hwfdefs: forall ids0,
+     let '(Opsem.mkEC F B cs tmn lc als) := EC in
+     F = (PI_f pinfo) ->
+     inscope_of_pc F B cs tmn = Some ids0 ->
+     wf_defs maxb pinfo TD M lc ids0 als ->
+     wf_defs maxb pinfo TD M' lc ids0 als)
+  (Hwflc: wf_lc M (@Opsem.Locals DGVs EC) -> wf_lc M' (Opsem.Locals EC))
+  (Hwf: wf_ExecutionContext maxb pinfo TD M EC),
+  wf_ExecutionContext maxb pinfo TD M' EC.
+Proof.
+  destruct EC. simpl. intros.
+  destruct Hwf as [J1 J2].
+  split; auto.
+    destruct (fdef_dec (PI_f pinfo) CurFunction); subst; auto.
+    destruct CurCmds.    
+      remember (inscope_of_tmn (PI_f pinfo) CurBB Terminator) as R.
+      destruct R; auto.
+
+      remember (inscope_of_cmd (PI_f pinfo) CurBB c) as R.
+      destruct R; auto.
+Qed.
+
+Lemma wf_ECStack_head_tail_cons__inv: forall maxb pinfo TD M lc ec1 ecs2,
+  wf_ECStack_head_tail maxb pinfo TD M lc (ec1::ecs2) ->
+  wf_ECStack_head_in_tail maxb pinfo TD M lc ec1 /\
+  wf_ECStack_head_tail maxb pinfo TD M lc ecs2.
+Proof.
+  intros.
+  split.
+    apply H; simpl; auto.
+    unfold wf_ECStack_head_tail in *. intros. apply H; simpl; auto.
+Qed.
+
+Lemma free_preserves_wf_ECStack_in_tail : forall maxb pinfo TD M  
+  M' mptr0 mptrs gl v (Hwfpi: WF_PhiInfo pinfo) lc
+  (Hgetop: Opsem.getOperandValue TD v lc gl = ret mptrs)
+  (Hin: mptr0 @ mptrs) (Hwfgl: wf_globals maxb gl)
+  (Hfree: free TD M mptr0 = ret M') ECs
+  (Hht: wf_ECStack_head_tail maxb pinfo TD M lc 
+          (List.map 
+             (fun ec => let '(Opsem.mkEC f _ _ _ lc _) := ec in (f, lc)) ECs))
+  (Hwf: wf_ECStack maxb pinfo TD M ECs),
+  wf_ECStack maxb pinfo TD M' ECs.
+Proof.
+  induction ECs; simpl; intros; auto.
+    destruct Hwf as [J1 [J2 J3]].
+    apply wf_ECStack_head_tail_cons__inv in Hht.
+    destruct Hht as [Hht1 Hht2].
+    split.
+      eapply impure_cmd_preserves_wf_EC_tail with (M:=M); eauto.
+        destruct a. intros. subst.
+        eapply free_preserves_wf_defs_in_tail; eauto.
+        eapply free_preserves_wf_lc; eauto.
+    split; auto.
+      eapply free_preserves_wf_ECStack_head_tail; eauto.
+(* Can this lemma be more generic by making free_preserves_mload_inv generic? *)
+Qed.
+
+Lemma free_preserves_wf_Mem : forall maxb TD M M' mptr0
+  (Hfree: free TD M mptr0 = ret M') 
+  (Hwf: wf_Mem maxb TD M),
+  wf_Mem maxb TD M'.
+Proof.
+  intros. destruct Hwf as [J1 J2].
+  split.
+    intros. 
+    eapply free_preserves_mload_inv in H; eauto.
+    apply J1 in H; auto.
+    admit. (* Mem Props *)
+  
+    admit. (* Mem Props *)
+Qed.
+
+Lemma free_preserves_wf_als : forall maxb TD M M' mptr0 als
+  (Hfree: free TD M mptr0 = ret M') 
+  (Hwf: wf_als maxb M als),
+  wf_als maxb M' als.
+Proof.
+  intros. destruct Hwf as [J1 J2].
+  split; auto.
+    intros. 
+    apply J2 in H; auto.
+    admit. (* Mem Props *)
+Qed.
+
+Lemma mstore_preserves_mload_inv: forall TD Mem' gptr ty al gvs0 Mem gv1 t
+  mp2 (H1 : mload TD Mem' gptr ty al = ret gvs0) align
+  (H2 : mstore TD Mem mp2 t gv1 align = Some Mem'),
+  Some gvs0 = gundef TD ty \/
+  gvs0 = gv1 \/
+  mload TD Mem gptr ty al = ret gvs0.
+Proof.
+  intros.
+  apply store_inv in H2.
+  destruct H2 as [b [ofs [J5 J4]]].
+  admit. (* mem prop *)
+Admitted.
+
+Lemma mstore_preserves_mload: forall TD Mem' gptr ty al gvs0 Mem gv1 t
+  mp2 (H1 : mload TD Mem gptr ty al = ret gvs0) align
+  (H2 : mstore TD Mem mp2 t gv1 align = Some Mem')
+  (Hna: no_alias mp2 gptr),
+  mload TD Mem' gptr ty al = ret gvs0.
+Proof.
+  admit. (* mem prop *)
+Admitted.
+
+Lemma mstore_preserves_mload': forall TD Mem' gptr ty al gvs0 Mem gv1 t
+  mp2 (H1 : mload TD Mem gptr ty al = ret gvs0) align
+  (H2 : mstore TD Mem mp2 t gv1 align = Some Mem'),
+  exists gvs1, mload TD Mem' gptr ty al = ret gvs1.
+Proof.
+  admit. (* mem prop *)
+Admitted.
+
+Lemma mstore_preserves_wf_defs_at_head : forall maxb pinfo TD M  
+  M' gl v als lc gvs1 gv1 t mp2 align mps2 vp
+  (Hgetop': Opsem.getOperandValue TD vp lc gl = ret mps2)
+  (Hgetop: Opsem.getOperandValue TD v lc gl = ret gvs1)
+  (Hinp: mp2 @ mps2) (Hin: gv1 @ gvs1) (Hwfgl: wf_globals maxb gl)
+  (Hst: mstore TD M mp2 t gv1 align = Some M')
+  ids0 (Hwfu: wf_use_at_head pinfo ids0 v) 
+  (Hwf: wf_defs maxb pinfo TD M lc ids0 als),
+  wf_defs maxb pinfo TD M' lc ids0 als.
+Proof.
+  intros. unfold wf_defs. 
+  intros gvsa Hpindom Hlkp.
+  assert (no_alias gv1 gvsa) as J.
+    eapply operand__no_alias_with__head with (mptrs:=gvs1); eauto.
+  assert (Hlkp':=Hlkp).
+  apply Hwf in Hlkp'; auto.
+  destruct Hlkp' as [J1 J2].
+  split; auto.
+    destruct J1 as [[mb [J11 J12]] [J4 [gv J3]]]; subst.
+    split; eauto.
+    split.
+      intros. 
+      eapply mstore_preserves_mload_inv in H; eauto.
+      destruct H as [H | [H | H]]; subst; eauto.
+        eapply undef_disjoint_with_runtime_alloca; eauto.
+
+      eapply mstore_preserves_mload'; eauto.
+Qed.
+
+Lemma mstore_preserves_wf_defs_in_tail : forall maxb pinfo TD M  
+  M' lc1 gl v als lc2 gvs1 gv1 t mp2 align mps2 vp
+  (Hgetop': Opsem.getOperandValue TD vp lc1 gl = ret mps2)
+  (Hgetop: Opsem.getOperandValue TD v lc1 gl = ret gvs1)
+  (Hinp: mp2 @ mps2) (Hin: gv1 @ gvs1) (Hwfgl: wf_globals maxb gl)
+  (Hst: mstore TD M mp2 t gv1 align = Some M')
+  (Hht: wf_ECStack_head_in_tail maxb pinfo TD M lc1 (PI_f pinfo, lc2))
+  ids0 (Hwf: wf_defs maxb pinfo TD M lc2 ids0 als),
+  wf_defs maxb pinfo TD M' lc2 ids0 als.
+Proof.
+  intros. unfold wf_defs. 
+  intros gvsa Hpindom Hlkp.
+  assert (Hlkp':=Hlkp).
+  apply Hwf in Hlkp'; auto.
+  destruct Hlkp' as [J1 J2].
+  split; auto.
+    clear J2.
+    destruct J1 as [[mb [J11 J12]] [J4 [gv J3]]]; subst.
+    split; eauto.
+    split.
+      intros.
+      eapply mstore_preserves_mload_inv in Hst; eauto.
+      destruct Hst as [G | [G | G]]; subst; eauto.
+        eapply undef_disjoint_with_runtime_alloca; eauto.
+        eapply operand__no_alias_with__tail; eauto.
+
+      exists gv. 
+      eapply mstore_preserves_mload; eauto.
+      eapply operand__no_alias_with__tail; eauto.
+Qed.
+
+Lemma mstore_preserves_wf_lc: forall TD M' M mp2 t gv1 align
+  (Hst: mstore TD M mp2 t gv1 align = Some M') lc
+  (Hwf: wf_lc M lc),
+  wf_lc M' lc.
+Proof.
+  unfold wf_lc.
+  intros.
+  apply Hwf in H.
+  apply store_inv in Hst.
+  destruct Hst as [blk' [ofs' [J1 J2]]].
+  admit. (* Mem Props *)
+Qed.
+
+Lemma mstore_preserves_wf_ECStack_head_tail: forall maxb pinfo ECs TD M 
+  gv1 align M' lc mp2 t gvs1 gl v1 (Hwfgl: wf_globals maxb gl) EC
+  (H0 : Opsem.getOperandValue TD v1 lc gl = Some gvs1)
+  (H1 : gv1 @ gvs1)
+  (Hst: mstore TD M mp2 t gv1 align = Some M') lc1 (Heq: lc1 = snd EC)
+  (Hht: wf_ECStack_head_tail maxb pinfo TD M lc (EC::ECs))
+  (Hwf: wf_ECStack_head_tail maxb pinfo TD M lc1 ECs),
+  wf_ECStack_head_tail maxb pinfo TD M' lc1 ECs.
+Proof.
+  intros.
+  unfold wf_ECStack_head_tail, wf_ECStack_head_in_tail.
+  intros.
+  assert (no_alias gv1 gvsa) as J.
+    eapply operand__no_alias_with__tail with (M:=M); eauto.
+      unfold wf_ECStack_head_in_tail.
+      intros. 
+      eapply Hht; eauto.
+      simpl. right. rewrite <- H2.
+      destruct ec0; auto.
+  eapply Hwf in H3; eauto.
+  destruct H3 as [[mb [J11 J12]] [J2 J3]]; subst.
+  split.
+    exists mb. split; auto. admit. (* MemProp *)
+  split; auto.
+    intros.
+    eapply mstore_preserves_mload_inv in Hst; eauto.
+    destruct Hst as [G | [G | G]]; subst; eauto.
+      eapply undef_disjoint_with_runtime_alloca; eauto.
+Qed.
+
+Lemma wf_ECStack_head_tail_cons__intro: forall maxb pinfo TD M lc ec1 ecs2,
+  wf_ECStack_head_in_tail maxb pinfo TD M lc ec1 ->
+  wf_ECStack_head_tail maxb pinfo TD M lc ecs2 ->
+  wf_ECStack_head_tail maxb pinfo TD M lc (ec1::ecs2).
+Proof.
+  intros.
+  unfold wf_ECStack_head_tail in *. 
+  intros. 
+  simpl in H1.
+  destruct H1 as [EQ | H1]; subst; auto.
+Qed.
+
+Lemma mstore_preserves_wf_ECStack_in_tail : forall maxb pinfo TD M mp2 t align M' gl vp
+  (Hwfgl: wf_globals maxb gl) lc gvs1 gv1 v1 (Hwfpi: WF_PhiInfo pinfo) mps2
+  (Hgetop': Opsem.getOperandValue TD vp lc gl = ret mps2)
+  (H0 : Opsem.getOperandValue TD v1 lc gl = Some gvs1)
+  (Hinp: mp2 @ mps2) (H1 : gv1 @ gvs1)
+  (Hst: mstore TD M mp2 t gv1 align = Some M') ECs
+  (Hht: wf_ECStack_head_tail maxb pinfo TD M lc 
+          (List.map 
+             (fun ec => let '(Opsem.mkEC f _ _ _ lc _) := ec in (f, lc)) ECs))
+  (Hwf: wf_ECStack maxb pinfo TD M ECs),
+  wf_ECStack maxb pinfo TD M' ECs.
+Proof.
+  induction ECs; simpl; intros; auto.
+    destruct Hwf as [J1 [J2 J3]].
+    apply wf_ECStack_head_tail_cons__inv in Hht.
+    destruct Hht as [Hht1 Hht2].
+    split.
+      eapply impure_cmd_preserves_wf_EC_tail with (M:=M); eauto.
+        destruct a. intros. subst.
+        eapply mstore_preserves_wf_defs_in_tail with (mps2:=mps2)(gvs1:=gvs1)
+          (v:=v1)(lc1:=lc)(vp:=vp) in Hst; eauto.
+        eapply mstore_preserves_wf_lc; eauto.
+    split; auto.
+      destruct a. simpl in *.
+      eapply mstore_preserves_wf_ECStack_head_tail 
+        with (EC:=(CurFunction, Locals)); eauto.
+        intros.
+        apply wf_ECStack_head_tail_cons__intro; auto.
+Qed.
+
+Lemma mstore_preserves_wf_Mem : forall maxb TD M mp2 t gv1 align M' gvs1 gl
+  (Hwfgl: wf_globals maxb gl) (lc:DGVMap) v1 (Hwflc: wf_lc M lc) 
+  (H0 : Opsem.getOperandValue TD v1 lc gl = Some gvs1)
+  (H1 : gv1 @ gvs1)
+  (Hst: mstore TD M mp2 t gv1 align = Some M')
+  (Hwf: wf_Mem maxb TD M),
+  wf_Mem maxb TD M'.
+Proof.
+  intros. destruct Hwf as [J1 J2].
+  assert (Mem.nextblock M = Mem.nextblock M') as EQ.
+    admit. (* Mem Props *)
+  rewrite EQ in *.
+  split; eauto.
+    intros.
+    eapply mstore_preserves_mload_inv in H; eauto.
+    destruct H as [G | [G | G]]; subst; eauto.
+      unfold gundef in G.
+      destruct (getTypeSizeInBits TD ty); tinv G.
+ 
+      eapply operand__lt_nextblock with (M:=M) in H0; eauto.
+        rewrite EQ in H0; auto.
+        rewrite EQ; auto.
+Qed.
+
+Lemma mstore_preserves_wf_als : forall TD M mp2 t gv1 align M' maxb als
+  (Hst: mstore TD M mp2 t gv1 align = Some M') 
+  (Hwf: wf_als maxb M als),
+  wf_als maxb M' als.
+Proof.
+  intros. destruct Hwf as [J1 J2].
+  split; auto.
+    intros. 
+    apply J2 in H; auto.
+    admit. (* Mem Props *)
+Qed.
+
+Lemma mstore_preserves_wf_ECStack_head_tail': forall maxb pinfo ECs TD M 
+  gv1 align M' lc mp2 t gvs1 gl v1 (Hwfgl: wf_globals maxb gl) 
+  (H0 : Opsem.getOperandValue TD v1 lc gl = Some gvs1)
+  (H1 : gv1 @ gvs1)
+  (Hst: mstore TD M mp2 t gv1 align = Some M') 
+  (Hwf: wf_ECStack_head_tail maxb pinfo TD M lc ECs),
+  wf_ECStack_head_tail maxb pinfo TD M' lc ECs.
+Proof.
+  intros.
+  unfold wf_ECStack_head_tail, wf_ECStack_head_in_tail.
+  intros.
+  assert (no_alias gv1 gvsa) as J.
+    eapply operand__no_alias_with__tail with (M:=M); eauto.
+      apply Hwf; auto.
+      rewrite <- H2.
+      destruct ec0; auto.
+  eapply Hwf in H3; eauto.
+  destruct H3 as [[mb [J11 J12]] [J2 J3]]; subst.
+  split. exists mb. split; auto. admit. (* MemProp *)
+  split; auto.
+    intros.
+    eapply mstore_preserves_mload_inv in Hst; eauto.
+    destruct Hst as [G | [G | G]]; subst; eauto.
+      eapply undef_disjoint_with_runtime_alloca; eauto.
+Qed.
+
+Lemma malloc_preserves_mload_inv: forall TD M M' mb align0 gn tsz 
+  (Hal : malloc TD M tsz gn align0 = ret (M', mb))
+  gptr gvs1 ty al 
+  (H : mload TD M' gptr ty al = ret gvs1),
+  mload TD M gptr ty al = ret gvs1 \/ ret gvs1 = gundef TD ty.
+Admitted.
+
+Lemma malloc_preserves_wf_ECStack_head_tail : forall maxb pinfo ECs TD M tsz gn 
+  align0 M' lc mb t id0
+  (Hmlc: malloc TD M tsz gn align0 = ret (M', mb))
+  (Hwf: wf_ECStack_head_tail maxb pinfo TD M lc ECs),
+  wf_ECStack_head_tail maxb pinfo TD M' 
+    (updateAddAL (GVsT DGVs) lc id0
+        ($ blk2GV TD mb # typ_pointer t $)) ECs.
+Proof.
+  intros.
+  unfold wf_ECStack_head_tail, wf_ECStack_head_in_tail.
+  intros.
+  eapply Hwf in H1; eauto.
+  destruct H1 as [[mb' [J11 J12]] [J2 J3]]; subst.
+  split. exists mb'. split; auto. admit. (* MemProp *)
+  split.
+    intros.
+    destruct (id_dec id0 id1); subst.
+      rewrite lookupAL_updateAddAL_eq in H1. inv H1.
+      admit. (* MemProp mb'<M.next=mb *)
+
+      rewrite <- lookupAL_updateAddAL_neq in H1; eauto.
+
+    intros.
+    eapply malloc_preserves_mload_inv in Hmlc; eauto.
+    destruct Hmlc as [G | G]; subst; eauto.
+      eapply undef_disjoint_with_runtime_alloca; eauto.
+Qed.
+
+Lemma malloc_preserves_wf_ECStack_in_tail : forall maxb pinfo TD M tsz gn align0 
+  (Hwfpi: WF_PhiInfo pinfo) M' mb 
+  (Hmlc: malloc TD M tsz gn align0 = ret (M', mb)) ECs 
+  (Hwf: wf_ECStack maxb pinfo TD M ECs),
+  wf_ECStack maxb pinfo TD M' ECs.
+Proof.
+  induction ECs; simpl; intros; auto.
+    destruct Hwf as [J1 [J2 J3]].
+    split.
+      eapply impure_cmd_preserves_wf_EC_tail with (M:=M); eauto.
+        destruct a. intros. subst.
+(*
+        eapply mstore_preserves_wf_defs_in_tail with (mps2:=mps2)(gvs1:=gvs1)
+          (v:=v1)(lc1:=lc)(vp:=vp) in Hst; eauto.
+        eapply mstore_preserves_wf_lc; eauto. 
+    split; auto.
+      destruct a. simpl in *.
+      eapply malloc_preserves_wf_ECStack_head_tail; eauto.
+        intros.
+        apply wf_ECStack_head_tail_cons__intro; auto.
+*)
+Admitted.
+
+Lemma malloc_preserves_wf_Mem : forall maxb TD M tsz gn align0 M' mb
+  (Hmlc: malloc TD M tsz gn align0 = ret (M', mb))
+  (Hwf: wf_Mem maxb TD M),
+  wf_Mem maxb TD M'.
+Proof.
+  intros. destruct Hwf as [J1 J2].
+  assert (Mem.nextblock M + 1 = Mem.nextblock M') as EQ.
+    admit. (* Mem Props *)
+  split.
+    rewrite <- EQ.
+    intros.
+    eapply malloc_preserves_mload_inv in H; eauto.
+    destruct H as [G | G]; subst; eauto.
+      apply J1 in G. omega.
+
+      unfold gundef in G.
+      destruct (getTypeSizeInBits TD ty); tinv G.
+ 
+    omega.
+Qed.
+
+Lemma alloca_preserves_wf_EC : forall maxb pinfo TD M tsz gn align0 M' mb 
+  als t id0 F B cs tmn lc v gns gl
+  (H : getTypeAllocSize TD t = ret tsz)
+  (H0 : Opsem.getOperandValue TD v lc gl = ret gns)
+  (H1 : gn @ gns)
+  (H2 : malloc TD M tsz gn align0 = ret (M', mb))
+  (HwfEC: wf_ExecutionContext maxb pinfo TD M 
+            {| Opsem.CurFunction := F;
+               Opsem.CurBB := B;
+               Opsem.CurCmds := insn_malloc id0 t v align0 :: cs;
+               Opsem.Terminator := tmn;
+               Opsem.Locals := lc;
+               Opsem.Allocas := als |}),
+  wf_ExecutionContext maxb pinfo TD M'
+   {| Opsem.CurFunction := F;
+      Opsem.CurBB := B;
+      Opsem.CurCmds := cs;
+      Opsem.Terminator := tmn;
+      Opsem.Locals := updateAddAL (GVsT DGVs) lc id0
+                        ($ blk2GV TD mb # typ_pointer t $);
+      Opsem.Allocas := mb :: als |}.
+Admitted.
+
+Lemma malloc_preserves_wf_als : forall maxb TD M M' tsz gn align0 mb als
+  (Hmalloc: malloc TD M tsz gn align0 = ret (M', mb)) 
+  (Hwf: wf_als maxb M als),
+  wf_als maxb M' (mb::als).
+Proof.
+  intros. destruct Hwf as [J1 J2].
+  split.
+    constructor; auto.
+      intro J. apply J2 in J.
+      admit. (* Mem Props *)
+
+    intros. 
+    simpl in H. 
+    destruct H as [H | H]; subst.
+      admit. (* Mem Props *)
+
+      apply J2 in H.
+      admit. (* Mem Props *)
+Qed.
+
+Lemma impure_cmd_updated_preserves_wf_EC : forall maxb pinfo TD M M' lc F B 
+  als als' tmn cs c0 l1 ps1 cs1' ifs S
+  (Heq: B = block_intro l1 ps1 (cs1' ++ c0 :: cs) tmn)
+  (HwfS: wf_system ifs S) los nts (Heq': TD = (los, nts)) Ps
+  (HMinS: moduleInSystemB (module_intro los nts Ps) S = true)
+  (HFinPs: InProductsB (product_fdef F) Ps = true)
+  (HBinF: blockInFdefB B F = true) id0
+  (Hid : getCmdID c0 = Some id0) gv3
+  (Hwfdefs: forall ids0,
+              F = (PI_f pinfo) ->
+              inscope_of_pc F B (c0::cs) tmn = Some ids0 ->
+              wf_defs maxb pinfo TD M lc ids0 als ->
+              wf_defs maxb pinfo TD M' 
+                (updateAddAL (GVsT DGVs) lc id0 gv3) (id0::ids0) als')
+  (Hwflc: wf_lc M lc -> wf_lc M' (updateAddAL (GVsT DGVs) lc id0 gv3)) EC
+  (Heq: EC = {| Opsem.CurFunction := F;
+               Opsem.CurBB := B;
+               Opsem.CurCmds := c0 :: cs;
+               Opsem.Terminator := tmn;
+               Opsem.Locals := lc;
+               Opsem.Allocas := als |})
+  (HwfEC: wf_ExecutionContext maxb pinfo TD M EC),
+  wf_ExecutionContext maxb pinfo TD M'
+    {| Opsem.CurFunction := F;
+       Opsem.CurBB := B;
+       Opsem.CurCmds := cs;
+       Opsem.Terminator := tmn;
+       Opsem.Locals := updateAddAL (GVsT DGVs) lc id0 gv3;
+       Opsem.Allocas := als' |}.
+Proof.
+  simpl. intros. subst.
+  destruct HwfEC as [J1 J2].
+  split; auto.
+  destruct (fdef_dec (PI_f pinfo) F); subst; auto.
+  remember (inscope_of_cmd (PI_f pinfo) 
+    (block_intro l1 ps1 (cs1' ++ c0 :: cs) tmn) c0) as R1. 
+  assert (HeqR1':=HeqR1).
+  unfold inscope_of_cmd, inscope_of_id in HeqR1'.
+
+  destruct R1; try solve [inversion J1].
+  repeat (split; try solve [auto]).
+      destruct cs; simpl_env in *.
+      SSSSCase "cs = nil".
+        assert (~ In (getCmdLoc c0) (getCmdsLocs cs1')) 
+          as Hnotin.
+          eapply preservation_helper1; eauto.
+
+        apply inscope_of_cmd_tmn in HeqR1; auto.
+        destruct HeqR1 as [ids2 [J1' J2']].
+        rewrite <- J1'.
+        assert (In c0 (cs1' ++ [c0])) as HinCs.
+          apply in_or_app. right. simpl. auto.
+        assert (Hwfc := HBinF).
+        eapply wf_system__wf_cmd with (c:=c0) in Hwfc; 
+          eauto.
+        assert (HwfF:=HFinPs). eapply wf_system__wf_fdef in HwfF; eauto.
+        rewrite Hid in J2'.
+        eapply wf_defs_eq; eauto.       
+
+      SSSSCase "cs <> nil".
+        assert (NoDup (getCmdsLocs (cs1' ++ [c0] ++ [c] ++ cs))) 
+          as Hnodup.
+          eapply preservation_helper2; eauto.
+
+        apply inscope_of_cmd_cmd in HeqR1; auto.
+        destruct HeqR1 as [ids2 [J1' J2']].        
+        rewrite <- J1'.
+        assert (In c0 (cs1' ++ [c0] ++ [c] ++ cs)) 
+          as HinCs.
+          apply in_or_app. right. simpl. auto.
+        assert (Hwfc := HBinF).
+        eapply wf_system__wf_cmd with (c:=c0) in Hwfc; 
+          eauto.
+        rewrite Hid in J2'. 
+        eapply wf_defs_eq; eauto.
+Qed.
+
+Lemma alloca_preserves_wf_defs_at_head : forall maxb pinfo TD M  
+  M' gl als lc t v
+  (Hwfgl: wf_globals maxb gl) mb id0 tmn align0 cs cs1' l1 ps1 F gn tsz
+  (Hal: malloc TD M tsz gn align0 = ret (M', mb)) (HwfM: wf_Mem maxb TD M)
+  (Hwflc : wf_lc M lc),
+  forall ids0,
+   F = PI_f pinfo ->
+   inscope_of_pc F
+     (block_intro l1 ps1 (cs1' ++ insn_alloca id0 t v align0 :: cs) tmn)
+     (insn_alloca id0 t v align0 :: cs) tmn = ret ids0 ->
+   wf_defs maxb pinfo TD M lc ids0 als ->
+   wf_defs maxb pinfo TD M'
+     (updateAddAL (GVsT DGVs) lc id0
+        ($ blk2GV TD mb # typ_pointer t $)) 
+     (id0 :: ids0) (mb :: als).
+Proof.
+  intros. unfold wf_defs. 
+  intros gvsa Hpindom Hlkp.
+  destruct (id_dec id0 (PI_id pinfo)); subst.
+    rewrite lookupAL_updateAddAL_eq in Hlkp.
+    inv Hlkp.
+    split.
+      split.
+        exists mb. admit. (* WF, MemProp *)
+      split.
+        intros.
+        assert (mload TD M gptr ty al = ret gvs1 \/
+                Some gvs1 = gundef TD ty) as J.
+          eapply malloc_preserves_mload_inv; eauto.
+        destruct J as [J | J].
+          destruct HwfM as [HwfM _].
+          admit. (* if gvs1 isnt ptr, done; else by HwfM *)
+
+          eapply undef_disjoint_with_runtime_alloca; eauto.
+
+        admit. (* MemProp by Hal. *)
+
+      intros.
+      unfold wf_non_alloca_GVs.
+      destruct (id_dec id0 (PI_id pinfo)); auto.
+      rewrite <- lookupAL_updateAddAL_neq in Hlk0; auto.
+      admit. (* if gvs1 isnt ptr, done; else by Hwflc *)
+
+    rewrite <- lookupAL_updateAddAL_neq in Hlkp; auto.
+    simpl in Hpindom.
+    destruct Hpindom as [Hpindom | Hpindom]; subst; try congruence.
+    assert (Hlkp':=Hlkp).
+    apply H1 in Hlkp; auto.
+    destruct Hlkp as [J1 J2].
+    split.
+      destruct J1 as [[mb' [J31 [J32 J33]]] [J4 [gv J5]]]; subst.
+      split.
+        exists mb'. split; auto. simpl. auto.
+      split.
+        intros.
+        assert (mload TD M gptr ty al = ret gvs1 \/
+                Some gvs1 = gundef TD ty) as J.
+          eapply malloc_preserves_mload_inv; eauto.
+        destruct J as [J | J]; eauto.
+          eapply undef_disjoint_with_runtime_alloca; eauto.
+
+        exists gv. admit. (* MemProp by Hal. *)
+
+      intros.
+      unfold wf_non_alloca_GVs.
+      destruct (id_dec id1 (PI_id pinfo)); auto.
+      destruct (id_dec id0 id1); subst.
+        rewrite lookupAL_updateAddAL_eq in Hlk0.
+        inv Hlk0.
+        admit. (* if gvsa isnt ptr, done; else by Hwflc *)
+
+        rewrite <- lookupAL_updateAddAL_neq in Hlk0; auto.
+        clear - Hpindom H0.
+        admit. (* sdom is acyclic *)
+Qed.
+
+Lemma malloc_preserves_wf_defs_at_head : forall maxb pinfo TD M  
+  M' gl als lc t v
+  (Hwfgl: wf_globals maxb gl) mb id0 tmn align0 cs cs1' l1 ps1 F gn tsz
+  (Hal: malloc TD M tsz gn align0 = ret (M', mb)) (HwfM: wf_Mem maxb TD M)
+  (Hwflc : wf_lc M lc),
+  forall ids0,
+   F = PI_f pinfo ->
+   inscope_of_pc F
+     (block_intro l1 ps1 (cs1' ++ insn_malloc id0 t v align0 :: cs) tmn)
+     (insn_alloca id0 t v align0 :: cs) tmn = ret ids0 ->
+   wf_defs maxb pinfo TD M lc ids0 als ->
+   wf_defs maxb pinfo TD M'
+     (updateAddAL (GVsT DGVs) lc id0
+        ($ blk2GV TD mb # typ_pointer t $)) 
+     (id0 :: ids0) als.
+Proof.
+  intros. unfold wf_defs. 
+  intros gvsa Hpindom Hlkp.
+  destruct (id_dec id0 (PI_id pinfo)); subst.
+    rewrite lookupAL_updateAddAL_eq in Hlkp.
+    inv Hlkp.
+    split.
+      split.
+        exists mb. admit. (* WF, MemProp *)
+      split.
+        intros.
+        assert (mload TD M gptr ty al = ret gvs1 \/
+                Some gvs1 = gundef TD ty) as J.
+          eapply malloc_preserves_mload_inv; eauto.
+        destruct J as [J | J].
+          destruct HwfM as [HwfM _].
+          admit. (* if gvs1 isnt ptr, done; else by HwfM *)
+
+          eapply undef_disjoint_with_runtime_alloca; eauto.
+
+        admit. (* MemProp by Hal. *)
+
+      intros.
+      unfold wf_non_alloca_GVs.
+      destruct (id_dec id0 (PI_id pinfo)); auto.
+      rewrite <- lookupAL_updateAddAL_neq in Hlk0; auto.
+      admit. (* if gvs1 isnt ptr, done; else by Hwflc *)
+
+    rewrite <- lookupAL_updateAddAL_neq in Hlkp; auto.
+    simpl in Hpindom.
+    destruct Hpindom as [Hpindom | Hpindom]; subst; try congruence.
+    assert (Hlkp':=Hlkp).
+    apply H1 in Hlkp; auto.
+    destruct Hlkp as [J1 J2].
+    split.
+      destruct J1 as [[mb' [J31 [J32 J33]]] [J4 [gv J5]]]; subst.
+      split.
+        exists mb'. split; auto. simpl. auto.
+      split.
+        intros.
+        assert (mload TD M gptr ty al = ret gvs1 \/
+                Some gvs1 = gundef TD ty) as J.
+          eapply malloc_preserves_mload_inv; eauto.
+        destruct J as [J | J]; eauto.
+          eapply undef_disjoint_with_runtime_alloca; eauto.
+
+        exists gv. admit. (* MemProp by Hal. *)
+
+      intros.
+      unfold wf_non_alloca_GVs.
+      destruct (id_dec id1 (PI_id pinfo)); auto.
+      destruct (id_dec id0 id1); subst.
+        rewrite lookupAL_updateAddAL_eq in Hlk0.
+        inv Hlk0.
+        admit. (* if gvsa isnt ptr, done; else by Hwflc *)
+
+        rewrite <- lookupAL_updateAddAL_neq in Hlk0; auto.
+        clear - Hpindom H0.
+        admit. (* sdom is acyclic *)
+Qed.
+
+Lemma malloc_preserves_wf_lc: forall TD M M' tsz gn align0 mb t id0 lc
+  (Hmalloc: malloc TD M tsz gn align0 = ret (M', mb)) 
+  (Hwf: wf_lc M lc),
+  wf_lc M' (updateAddAL (GVsT DGVs) lc id0 ($ blk2GV TD mb # typ_pointer t $)).
+Proof.
+  unfold wf_lc.
+  intros.
+  destruct (id_dec id0 id1); subst.
+    rewrite lookupAL_updateAddAL_eq in H.
+    admit. (* Mem Props *)
+
+    rewrite <- lookupAL_updateAddAL_neq in H; auto.
+    apply Hwf in H.
+    admit. (* Mem Props *)
+Qed.
+
+Ltac simpl_ctx Hinv HwfS1 :=
+  destruct Hinv as 
+    [_ [HwfSystem [HmInS [Hnonempty [
+     [Hreach1 [HBinF1 [HFinPs1 [_ [_ [l1 [ps1 [cs1' Heq1]]]]]]]] 
+     [HwfEC0 HwfCall]
+    ]]]]]; subst;
+  fold (@OpsemPP.wf_ECStack DGVs) in HwfEC0;
+  destruct HwfS1 as [[HwfEC [HwfECs Hwfht]] [Hnonup1 HwfM1]].
+
 Lemma preservation : forall maxb pinfo cfg S1 S2 tr
   (Hinv: OpsemPP.wf_State cfg S1)
   (Hwfg: wf_globals maxb ((OpsemAux.Globals cfg)))
@@ -1273,6 +1991,7 @@ Case "sBop".
   eapply preservation_pure_cmd_updated_case in HwfS1; try solve [simpl; eauto]; 
     eauto.
     eapply BOP__wf_GVs_in_EC; eauto.
+      admit. (* WF *)
 Case "sFBop". admit.
 Case "sExtractValue". admit. 
 (* tricky case, 
@@ -1281,12 +2000,16 @@ Case "sInsertValue". admit.
 (* tricky case, 
    we need to ensure that we are not inserting aliased values *)
 Case "sMalloc". 
-  destruct HwfS1 as [[HwfEC [HwfECs Hwfht]] [Hnonup1 HwfM1]].
+  simpl_ctx Hinv HwfS1.
   split.
     split.
-      eapply malloc_preserves_wf_EC in H2; eauto.
+      eapply impure_cmd_updated_preserves_wf_EC; eauto.
+        intros. subst.
+        apply wf_EC__wf_lc in HwfEC.
+        eapply malloc_preserves_wf_defs_at_head with (tmn:=tmn); eauto.
+        eapply malloc_preserves_wf_lc; eauto.
     split.
-      eapply malloc_preserves_wf_ECStack in H2; eauto.
+      eapply malloc_preserves_wf_ECStack_in_tail in H2; eauto.
       eapply malloc_preserves_wf_ECStack_head_tail in H2; eauto.
   split.
     eapply malloc_preserves_wf_als in H2; eauto.
@@ -1295,26 +2018,32 @@ Case "sMalloc".
     eapply malloc_preserves_wf_Mem in H2; eauto.
 
 Case "sFree". 
-  destruct HwfS1 as [[HwfEC [HwfECs Hwfht]] [Hnonup1 HwfM1]].
-  assert (wf_lc Mem lc) as Hwflc.
-    apply wf_EC__wf_lc in HwfEC; auto.
+  simpl_ctx Hinv HwfS1.
   split.
     split.
-      eapply free_preserves_wf_EC in H1; eauto.
+      eapply impure_cmd_non_updated_preserves_wf_EC with (M:=Mem); eauto.
+        intros. subst.
+        eapply free_preserves_wf_defs_at_head; eauto.
+          admit. (* WF PhiInfo *)
+        eapply free_preserves_wf_lc; eauto.
     split.
-      eapply free_preserves_wf_ECStack in H1; eauto.
+      eapply free_preserves_wf_ECStack_in_tail in H1; eauto.
       eapply free_preserves_wf_ECStack_head_tail in H1; eauto.
   split.
     eapply free_preserves_wf_als in H1; eauto.
     eapply free_preserves_wf_Mem in H1; eauto.
 
 Case "sAlloca". 
-  destruct HwfS1 as [[HwfEC [HwfECs Hwfht]] [Hnonup1 HwfM1]].
+  simpl_ctx Hinv HwfS1.
   split.
     split.
-      eapply alloca_preserves_wf_EC in H2; eauto.
-    split.
-      eapply malloc_preserves_wf_ECStack in H2; eauto.
+      eapply impure_cmd_updated_preserves_wf_EC; eauto.
+        intros. subst.
+        apply wf_EC__wf_lc in HwfEC.
+        eapply alloca_preserves_wf_defs_at_head; eauto.
+        eapply malloc_preserves_wf_lc; eauto.
+    split.       
+      eapply malloc_preserves_wf_ECStack_in_tail in H2; eauto.
       eapply malloc_preserves_wf_ECStack_head_tail in H2; eauto.
   split.
     eapply malloc_preserves_wf_als in H2; eauto.
@@ -1323,35 +2052,45 @@ Case "sAlloca".
 Case "sLoad". 
   eapply preservation_pure_cmd_updated_case in HwfS1; try solve [simpl; eauto]; 
     eauto.
-    destruct HwfS1 as [[[_ Hwflc] _] _]. 
+    destruct HwfS1 as [[[_ Hwflc] _] [_ HwfM]]. 
     eapply mload__wf_GVs_in_EC; eauto using wf_EC__wf_lc.
-
+      admit. (* WF *)
 Case "sStore". 
-  destruct HwfS1 as [[HwfEC [HwfECs Hwfht]] [Hnonup1 HwfM1]].
+  simpl_ctx Hinv HwfS1.
   assert (wf_lc Mem lc) as Hwflc.
     apply wf_EC__wf_lc in HwfEC; auto.
   split.
     split.
-      eapply mstore_preserves_wf_EC with (gvs1:=gvs1) in H3; eauto.
+      eapply impure_cmd_non_updated_preserves_wf_EC with (M:=Mem); eauto.
+        intros. subst.
+        eapply mstore_preserves_wf_defs_at_head with (gvs1:=gvs1) in H3; eauto.
+          admit. (* WF PhiInfo *)
+        eapply mstore_preserves_wf_lc; eauto.
     split.
-      eapply mstore_preserves_wf_ECStack in H3; eauto.
-      eapply mstore_preserves_wf_ECStack_head_tail in H3; eauto.
+      eapply mstore_preserves_wf_ECStack_in_tail with (gvs1:=gvs1) in H3; eauto.
+      eapply mstore_preserves_wf_ECStack_head_tail' with (gvs1:=gvs1) in H3; 
+        eauto.
   split.
     eapply mstore_preserves_wf_als in H3; eauto.
-    eapply mstore_preserves_wf_Mem in H3; eauto.
+    eapply mstore_preserves_wf_Mem with (gvs1:=gvs1) in H3; eauto.
 
 Case "sGEP". 
   eapply preservation_pure_cmd_updated_case in HwfS1; try solve [simpl; eauto]; 
     eauto.
-    destruct HwfS1 as [[[_ Hwflc] _] _]. 
+    destruct HwfS1 as [[[_ Hwflc] _] [_ [_ HwfM]]]. 
     eapply GEP__wf_GVs_in_EC; eauto using wf_EC__wf_lc.
+      admit. (* WF PI *)
+      admit. (* WF *)
 
 Case "sTrunc". admit.
 Case "sExt". admit.
 Case "sCast". 
   eapply preservation_pure_cmd_updated_case in HwfS1; try solve [simpl; eauto]; 
     eauto.
+    destruct HwfS1 as [[[_ Hwflc] _] [_ [_ HwfM]]]. 
     eapply CAST__wf_GVs_in_EC; eauto.
+      admit. (* WF PI *)
+      admit. (* WF *)
 
 Case "sIcmp". admit.
 Case "sFcmp". admit.
@@ -1451,3 +2190,4 @@ Qed.
 *** coq-prog-args: ("-emacs-U" "-I" "~/SVN/sol/vol/src/Vellvm/monads" "-I" "~/SVN/sol/vol/src/Vellvm/ott" "-I" "~/SVN/sol/vol/src/Vellvm/compcert" "-I" "~/SVN/sol/theory/metatheory_8.3" "-impredicative-set") ***
 *** End: ***
  *)
+
